add graph

theories/Graph.v
@@ -9,100 +9,160 @@ Unset Printing Implicit Defensive.
 Require Import Program. 
 Require Import Lia.
 
-Fixpoint unfold_top_recs_aux (U : countType) (n : nat) (g : gType U) :=
-if n is n'.+1 then
-  if g is GRec g' then unfold_top_recs_aux n' (g'[g])
-  else g
-else g.
+Ltac uf name := rewrite /name -/name.
 
-Fixpoint mu_height (U : countType) (g : gType U) :=
+Section Enumeration.
+Variable U : countType.
+Implicit Type g : gType U.
+Fixpoint gType_size g :=
 match g with
-| GRec g0 => 1 + (mu_height g0)
+ | GMsg a u g0 => 1 + (gType_size  g0)
+ | GRec g0 => 1 + (gType_size g0)
+ | GBranch a gs => 1 + (sumn (map gType_size gs))
+ | GEnd => 1
+(* | GPar g0 g1 => 1 + (gType_size g0) + (gType_size g1)*)
+ | GVar n => 1
+end.
+
+Fixpoint mu_height g :=
+match g with
+| GRec g0 => (mu_height g0).+1
 | _ => 0
 end.
 
-Definition unfold_top_recs (U : countType) (g : gType U) := 
- unfold_top_recs_aux (mu_height g) g.
+Fixpoint unf_recs_aux n g  :=
+if n is n'.+1 then
+  if g is GRec g' then unf_recs_aux n' (g'[g])
+  else g
+else g.
+
+Notation unf_recs g := (unf_recs_aux (mu_height g) g).
 
 
-Section AGType.
-Variable (U : countType).
-Definition act_of_gType (g : gType U) :=
-match (unfold_top_recs g) with 
+Lemma contractive_mu_height : forall (g0 g1 : gType U) i, contractive_i (S i) g0 -> mu_height (substitution i g0 g1) = mu_height g0.
+Proof. 
+elim; try solve [by rewrite /=].
+- rewrite /=. intros. case : (eqVneq n i) H. move=>->. by rewrite ltnn. by rewrite /=. 
+- intros. rewrite /=. f_equal. apply H. done. 
+Qed.
+
+
+Lemma bound_lt : forall (g : gType U) i j, i < j -> bound_i i g -> bound_i j g.
+Proof. 
+elim/gType_ind_list.
+- rewrite /=;auto. move=>n i j.  move=> /leP H /ltP H1. apply/ltP.  lia. 
+- rewrite /=;auto. intros. apply : (@H i.+1 j.+1); done. 
+- rewrite /=;auto. 
+- intros. move : H1. rewrite /=.  move/allP=>H2. apply/allP. move=> l' Hin. move : (H2 l' Hin). 
+  apply H;auto. 
+- intros. simpl in H. done.
+- rewrite /=. intros. case : H1 H3. rewrite inE. case/orP. move/eqP=>->. eauto. 
+  eauto.
+Qed.
+
+
+Lemma bound_0 : forall (g : gType U) j, bound g -> bound_i j g.
+Proof.
+intros. case : j. done. intros. apply  : (@bound_lt _ 0). done. done.
+Qed.
+
+Lemma bound_subst : forall (g g': gType U) i, bound_i (S i) g -> bound g' -> bound_i i (substitution i g g').
+Proof.
+elim/gType_ind_list.
+-  rewrite /=;intros;case : (eqVneq n i).
+   move=><-. apply bound_0. done. rewrite /bound_i. move : H. move=> /ltP H1 /eqP H2. 
+   apply/ltP. lia. 
+- rewrite /=. done. 
+- rewrite /=. intros. apply H. done. done.
+- rewrite /=. intros. auto. 
+- rewrite /=. intros. move : (allP H0)=> H2. apply/allP. move => l' /mapP. case. intros. 
+  subst. apply H;auto.
+- rewrite /=. move => g. by rewrite in_nil. 
+- move => g H l IH g0. rewrite inE. case/orP. move/eqP =>->; auto. auto. 
+Qed.
+
+Lemma contractive_lt : forall (g : gType U) i j, j < i -> contractive_i i g -> contractive_i j g.
+Proof.
+elim;auto.
+- rewrite /=. move => n i j. move/ltP=> + /leP;intros.  apply/leP. lia. 
+- move => g H.  rewrite /=. intros. have : j.+1 < i.+1. apply/ltP. move : H0. move/ltP. lia. eauto. 
+Qed.
+
+Lemma contractive_0 : forall (g : gType U) i,  contractive_i i g -> contractive g.
+Proof.
+move=> g. case. done. intros.  apply : contractive_lt; last eauto. done.
+Qed.
+
+Lemma bound_contractive_subst : forall (g g': gType U) i j, bound_i (S i) g -> contractive_i j g -> bound g' -> (forall j, contractive_i j g') -> 
+contractive_i j (substitution i g g').
+Proof.
+elim/gType_ind_list; (try solve [rewrite /= ;auto]).
+- rewrite/=. move => v g' i j. case : (eqVneq v i).  done. simpl. done.
+- rewrite /=. intros. apply/allP. move=> gsub /mapP. case. intros. subst. 
+  apply H;auto. auto using (allP H0), (allP H1). auto using (allP H1). 
+- rewrite /=. intros.  move : H1 H2 H3. rewrite inE. case/orP. move/eqP=>->. 
+  eauto. eauto. 
+Qed.
+
+Lemma bound_cont_eq : forall (g : gType U) i, bound_i i g -> contractive_i i g -> (forall j, contractive_i j g).
+Proof.
+elim; rewrite/=;auto.
+- rewrite /=. move => v i /ltP + /leP. lia. 
+- rewrite /=. intros. eauto. 
+Qed.
+
+Lemma unf_recs_helper : forall n g, bound g -> contractive g -> mu_height (unf_recs_aux n g) = (mu_height g) - n.
+Proof.
+elim. 
+- intros. rewrite /=. Search _ (_ - _). elim : (mu_height g);done. 
+- intros. rewrite /=. case : g H0 H1; rewrite /= //=.
+intros. rewrite subSS. rewrite H. rewrite contractive_mu_height //=.
+- auto using bound_subst. 
+- apply bound_contractive_subst;auto. apply : contractive_0. eauto.  apply : bound_cont_eq. 
+ eauto. rewrite /=. done. 
+Qed.
+
+(*unf_recs unfolds all mu's, if g is bound and contractive, this is only relevant
+ for the specification of linearity
+ We trust that act_of_g and g_next do as intended*)
+Lemma unf_recs_fully : forall g, bound g -> contractive g -> mu_height (unf_recs g) = 0. 
+Proof. 
+intros. rewrite unf_recs_helper //=. rewrite subnE /=.
+remember (mu_height g). clear Heqn. elim : n. done. done. 
+Qed.
+
+Definition act_of_g g :=
+match unf_recs g with 
 | GMsg a _ _ => Some a
 | GBranch a _ => Some a
 | _ => None
 end.
 
-Definition has_prefix (g : gType U) := act_of_gType g != None.
-
-Inductive agType := AGType g of has_prefix g.
-
-Definition agType_project ag := let: AGType g _ := ag in g.
-Canonical agType_subType := [subType for agType_project]. 
-Definition agType_eqMixin := Eval hnf in [eqMixin of agType by <:].
-Canonical agType_eqType := Eval hnf in EqType agType agType_eqMixin.
-Definition agType_choiceMixin := [choiceMixin of agType by <:].
-Canonical agType_choiceType :=
-  Eval hnf in ChoiceType agType agType_choiceMixin.
-Definition agType_countMixin := [countMixin of agType by <:].
-Canonical agType_countType := Eval hnf in CountType agType agType_countMixin.
-Canonical agType_subCountType := [subCountType of agType].
-
-Lemma action_exists : forall (ag : agType), { a : action | act_of_gType (agType_project ag) = Some a }.
-Proof. Admitted.
-
-Definition action_of_ag (ag : agType) := let: exist a _ := action_exists ag in a.
-
-
-End AGType.
-Check agType.
-Definition gType_of_agType : forall (U : countType), agType U -> gType U := agType_project.
-Coercion gType_of_agType : agType >-> gType.
-Definition action_of_agType : forall (U : countType), agType U -> action := action_of_ag.
-Coercion action_of_ag : agType >-> action.
-
-
-Section Graph.
-Variable (U : countType). 
-Check foldl.
-
-Definition g_next (g : gType U) : seq (gType U) :=
-match g with 
+Definition g_next g :=
+match unf_recs g with 
 | GMsg _ _ g0 => [::g0]
 | GBranch _ gs => gs
-| GPar g0 g1 => [::g0;g1]
-| GRec g0 => [::unfold_top_recs g0]
 | _ => [::]
 end.
 
-Definition ag_next (ag : agType U) : seq (agType U) := 
- pmap insub (g_next ag).
-
-Fixpoint agType_enum_aux (n : nat) (ags : seq (agType U)) (ag : agType U) : seq (agType U) :=
+Fixpoint gType_enum_aux n gs g :=
 if n is n'.+1 then
-  if ag \in ags then ags
-   else foldl (agType_enum_aux n') (ag::ags) (ag_next ag)
-else ags.
+  if g \in gs then gs
+   else foldl (gType_enum_aux n') (g::gs) (g_next g)
+else gs.
 
-Fixpoint gType_size (g : gType U) :=
-match g with
- | GMsg a u g0 => 1 + (gType_size g0)
- | GRec g0 => 1 + (gType_size g0)
- | GBranch a gs => 1 + (sumn (map gType_size gs))
- | GEnd => 1
- | GPar g0 g1 => 1 + (gType_size g0) + (gType_size g1)
- | GVar n => 1
-end. 
-
-Definition agType_enum (ag : agType U) := agType_enum_aux (gType_size ag) ([::]) ag.
+Definition gType_enum (g : gType U) := undup (filter (fun g_f : gType U => act_of_g g_f != None) (gType_enum_aux (gType_size g) nil g)).
+End Enumeration.
+Arguments g_next {_}.
+Arguments gType_enum {_}.
 
 Section Node.
-Variable ag : agType U.
+Variable U : countType.
+Variable g : gType U.
 
-Inductive node := Node ag_n of ag_n \in (agType_enum ag).
+Inductive node := Node (g_n : gType U) of g_n \in gType_enum g. 
 
-Definition node_project n := let: Node ag_n _ := n in ag_n.
+Definition node_project (n : node) : gType U := let: Node p _ := n in p. 
 Canonical node_subType := [subType for node_project]. 
 Definition node_eqMixin := Eval hnf in [eqMixin of node by <:].
 Canonical node_eqType := Eval hnf in EqType node node_eqMixin.
@@ -113,61 +173,91 @@ Definition node_countMixin := [countMixin of node by <:].
 Canonical node_countType := Eval hnf in CountType node node_countMixin.
 Canonical node_subCountType := [subCountType of node].
 
-Definition node_next (n : node) : seq node := 
- pmap insub (ag_next (node_project n)).
-
-Lemma in_node (n : node) : (node_project n) \in (agType_enum ag).
-Proof. Admitted.
-
-(*Lemma node_inj : injective node_project. 
-Proof. Admitted.*)
-
-Definition node_enum : seq node := pmap insub (agType_enum ag).
-
-Lemma node_enum_uniq : uniq node_enum.
-Proof. Admitted.
+Definition node_enum : seq node := pmap insub (gType_enum g).
 
 Lemma mem_node_enum n : n \in node_enum.
-Proof. Admitted.
+Proof. rewrite /node_enum. rewrite mem_pmap_sub. 
+case : n. intros. rewrite /=. done. 
+Qed.
 
+Lemma node_enum_uniq : uniq node_enum.
+Proof. rewrite pmap_sub_uniq //=. 
+rewrite /gType_enum. apply undup_uniq. 
+Qed.
+
+Lemma in_undup : forall (A : eqType) (l : seq A) (a : A), a \in (undup l) -> a \in l.
+Proof. 
+move => A. elim. 
+- by rewrite /=.
+- move => a l IH a0.  rewrite /=. case: (@idP (a \in l)). 
+ + intros. rewrite /=. rewrite inE. case : (eqVneq a0 a). done. 
+   rewrite /=. auto. 
+ + move => H. rewrite inE. case/orP. move/eqP=>->. by rewrite inE eqxx.
+  move/IH. rewrite inE. move=>->. apply/orP;auto. 
+Qed.
+
+Lemma action_exists : forall n, { a : action | act_of_g (node_project n) = Some a }.
+Proof. 
+elim. rewrite /gType_enum. move => gn i. move : (in_undup i). rewrite mem_filter. move/andP. case. 
+intros. destruct (act_of_g gn) eqn:Heqn. eauto.  done. 
+Qed.
+
+Definition act_of_n (n : node) := let: exist a _ := action_exists n in a. 
 
 Definition node_finMixin := Eval hnf in UniqFinMixin node_enum_uniq mem_node_enum.
 Canonical node_finType := Eval hnf in FinType node node_finMixin.
 Canonical node_subFinType := Eval hnf in [subFinType of node].
-
 End Node.
-End Graph.
 Arguments Node {_}.
-Check node_next.
-Arguments node_next {_} {_}.
-
-Definition agType_of_node : forall (U : countType) (g : agType U), node g -> agType U := node_project.
-Coercion agType_of_node : node >-> agType.
+Arguments gType_enum {_}.
+Coercion act_of_n : node >-> action. 
+Coercion node_project : node >-> gType.
 
 Section Order.
 Variable (U : countType). 
+Variable (g : gType U).
 
 Definition action_from (a : action) := let : Action p0 _ _ := a in p0.
 Definition action_to (a : action) := let : Action _ p1 _ := a in p1.
 Definition action_ch (a : action) := let : Action _ _ c := a in c.
+Definition same_ch (a0 a1 : action) := action_ch a0 == action_ch a1.
 
-Variable (ag : agType U).
+Definition opt_rel (g0 g1 : gType U) (P : rel action) :=
+if act_of_g g0 is Some a0
+  then if act_of_g g1 is Some a1
+    then P a0 a1
+  else false 
+else false.
 
-Definition II_rel (n0 n1 : node ag) := (action_to n0 == action_to n1).
-Definition IO_rel (n0 n1 : node ag) := (action_to n0 == action_from n1).
-Definition OO_rel (n0 n1 : node ag) := (action_from n0 == action_from n1) && (action_ch n0 == action_ch n1).
+Definition II_aux (a0 a1 : action) := (action_to a0 == action_to a1).
+Definition II (n0 n1 : node g) := (grel g_next n0 n1) && II_aux n0 n1.
+Definition II_spec (g0 g1 : gType U) := (grel g_next g0 g1) && opt_rel g0 g1 II_aux. 
 
-Definition in_dep (n0 n1 : node ag) := [exists n', connect IO_rel n0 n' && II_rel n' n1] || II_rel n0 n1.
-Definition out_dep (n0 n1 : node ag) := connect (fun n0 n1 => OO_rel n0 n1 || IO_rel n0 n1) n0 n1.
-End Order.
-Arguments in_dep {_} {_}.
-Arguments out_dep {_} {_}.
+Definition IO_aux (a0 a1 : action) := (action_to a0 == action_from a1).
+Definition IO (n0 n1 : node g) := (grel g_next n0 n1) && IO_aux n0 n1.
+Definition IO_spec (g0 g1 : gType U) := (grel g_next g0 g1) && opt_rel g0 g1 IO_aux. 
 
-Section Linear.
-Variable (U : countType).
+Definition OO_aux (a0 a1 : action) := (action_from a0 == action_from a1) && (action_ch a0 == action_ch a1).
+Definition OO (n0 n1 : node g) := (grel g_next n0 n1) && OO_aux n0 n1.
+Definition OO_spec (g0 g1 : gType U) := (grel g_next g0 g1) && opt_rel g0 g1 OO_aux. 
+
+Definition in_dep (n0 n1 : node g) := [exists n', connect IO n0 n' && II n' n1] || II n0 n1. 
+Definition in_dep_spec (g0 g1 : gType U) := (exists (g' : gType U), (exists2 p, path IO_spec g0 p & g' = last g0 p) /\ II_spec g' g1) 
+                                      \/ II_spec g0 g1.
 
 
-Definition linear (g : gType U) := 
-if insub g is Some ag then [forall n0 : node ag, forall (n1 : node ag | action_ch n0 == action_ch n1), in_dep n0 n1 && out_dep n0 n1]
-                      else true.
+Definition OO_IO (n n' : node g) := OO n n' || IO n n'.
+Definition OO_IO_spec (g g' : gType U) := OO_spec g g' || IO_spec g g'.
+Definition out_dep (n0 n1 : node g) := connect OO_IO n0 n1. 
+Definition out_dep_spec(g0 g1 : gType U) := exists2 p, path OO_IO_spec g0 p & g1 = last g0 p.
 
+Definition adjacent_rel (n0 n1 : node g) := (grel g_next) n0 n1.
+Definition linear := [forall n0 : node g, forall (n1 : node g | connect adjacent_rel n0 n1 && same_ch n0 n1), in_dep n0 n1 && out_dep n0 n1].
+Definition linear_spec := 
+forall (g0 g1 : gType U), (exists2 p, path (grel g_next) g p & g0 = last g p) ->
+                     (exists2 p, path (grel g_next) g0 p & g1 = last g0 p) ->
+  opt_rel g0 g1 same_ch -> bound g -> contractive g -> in_dep_spec g0 g1 /\ out_dep_spec g0 g1.
+
+Lemma linearP : reflect linear_spec linear.
+Proof. Admitted.
+End Order. 
